Add support for entities and concepts. The latter is incomplet

ref_impl/src/verifier/testing/simple_test.ts
@@ -1,0 +1,19 @@
+import { UnionType, IntType, TypeExpr, BoolType, NoneType } from "../type_expr"
+
+let a = new UnionType(new Set<TypeExpr>([new BoolType(), new IntType(), new NoneType()]));
+let b = new UnionType(new Set<TypeExpr>([new BoolType(), new IntType()]));
+
+function subsetOf(a: UnionType, b: UnionType) {
+
+    for(let element of a.elements){
+        for(let element2 of b.elements){
+            if(element.equalTo(element2)){
+                
+            }
+        }
+    }
+}
+
+console.log(subsetOf(a, b));
+
+
