ref_impl/src/verifier/NSMain__main_main.fst
@@ -1,6 +1,12 @@
 module NSMain__main_main
 open BosqueOption
 
+val nSMain__identityUnion : (x:bosqueTerm{subtypeOf (BUnionType BBoolType (BUnionType BIntType (BUnionType BNoneType (BTypeStringType BAnyType)))) (getType x)}) -> Tot (x:bosqueTerm{subtypeOf (BUnionType BBoolType (BUnionType BIntType (BUnionType BNoneType (BTypeStringType BAnyType)))) (getType x)})
+let nSMain__identityUnion x = 
+    let __ir_ret__ = x in 
+        let _return_ = __ir_ret__ in 
+            _return_
+
 val nSMain__max : (x:bosqueTerm{subtypeOf (BUnionType BIntType BNoneType) (getType x)}) -> (x:bosqueTerm{isInt x}) -> Tot (x:bosqueTerm{isInt x})
 let nSMain__max x y = 
     let __tmp_0 = true in 
@@ -22,58 +28,54 @@ let nSMain__max x y =
                             let _return_ = __ir_ret___3 in 
                                 _return_
 
-val nSMain__identityUnion : (x:bosqueTerm{subtypeOf (BUnionType BBoolType (BUnionType BIntType (BUnionType BNoneType (BTypeStringType BAnyType)))) (getType x)}) -> Tot (x:bosqueTerm{subtypeOf (BUnionType BBoolType (BUnionType BIntType (BUnionType BNoneType (BTypeStringType BAnyType)))) (getType x)})
-let nSMain__identityUnion x = 
-    let __ir_ret__ = x in 
-        let _return_ = __ir_ret__ in 
-            _return_
-
-val nSMain__identityTupleOptional : (x:bosqueTerm{subtypeOf (BUnionType (BTupleType false 1 (SCons BIntType SNil)) (BUnionType (BTupleType false 3 (SCons BIntType (SCons BBoolType (SCons BIntType SNil)))) (BTupleType true 4 (SCons BIntType (SCons BBoolType (SCons BIntType (SCons BBoolType SNil))))))) (getType x)}) -> Tot (x:bosqueTerm{subtypeOf (BUnionType (BTupleType false 1 (SCons BIntType SNil)) (BUnionType (BTupleType false 3 (SCons BIntType (SCons BBoolType (SCons BIntType SNil)))) (BTupleType true 4 (SCons BIntType (SCons BBoolType (SCons BIntType (SCons BBoolType SNil))))))) (getType x)})
+val nSMain__identityTupleOptional : (x:bosqueTerm{subtypeOf (BUnionType (BTupleType false 3 (SCons BIntType (SCons BBoolType (SCons BIntType SNil)))) (BTupleType true 4 (SCons BIntType (SCons BBoolType (SCons BIntType (SCons BBoolType SNil)))))) (getType x)}) -> Tot (x:bosqueTerm{subtypeOf (BUnionType (BTupleType false 3 (SCons BIntType (SCons BBoolType (SCons BIntType SNil)))) (BTupleType true 4 (SCons BIntType (SCons BBoolType (SCons BIntType (SCons BBoolType SNil)))))) (getType x)})
 let nSMain__identityTupleOptional x = 
     let __ir_ret__ = x in 
         let _return_ = __ir_ret__ in 
             _return_
 
-val nSMain__identity : (x:bosqueTerm{isTuple true 1 (SCons (BTypeStringType BAnyType) SNil)}) -> Tot (x:bosqueTerm{isTuple true 1 (SCons (BTypeStringType BAnyType) SNil)})
-let nSMain__identity x = 
+val nSMain__identityOpenTuple : (x:bosqueTerm{isTuple true 1 (SCons (BTypeStringType BAnyType) SNil)}) -> Tot (x:bosqueTerm{isTuple true 1 (SCons (BTypeStringType BAnyType) SNil)})
+let nSMain__identityOpenTuple x = 
     let __ir_ret__ = x in 
         let _return_ = __ir_ret__ in 
             _return_
 
 val nSMain__main : (x:bosqueTerm{isInt x})
 let nSMain__main  = 
-    let s = "hello1" in 
+    let string_test = "string_test" in 
         let _LoadConstTypeString = 0 in 
-            let s1 = __tmp_1 in 
+            let player1 = __tmp_1 in 
                 let n = none in 
                     let __tmp_3 = (Mktuple__2 10 30) in 
-                        let x = __tmp_3 in 
-                            let y = 20 in 
-                                let _MIRAccessFromIndex = 0 in 
-                                    let __tmp_7 = (nSMain__max __tmp_10 y) in 
-                                        let z = __tmp_7 in 
-                                            let __tmp_25 = (Mktuple__2 1 1) in 
-                                                let __tmp_12 = (Mktuple__16 1 1 1 1 1 1 1 1 1 1 1 1 __tmp_25 "hello" false true) in 
-                                                    let x2 = __tmp_12 in 
-                                                        let __tmp_31 = (Mkrecord__f_g 1 2) in 
-                                                            let x3 = __tmp_31 in 
+                        let xTuple2 = __tmp_3 in 
+                            let __tmp_19 = (Mktuple__2 1 1) in 
+                                let __tmp_6 = (Mktuple__16 1 1 1 1 1 1 1 1 1 1 1 1 __tmp_19 "hello" false true) in 
+                                    let x2 = __tmp_6 in 
+                                        let __tmp_25 = (Mkrecord__f_g 1 2) in 
+                                            let xRecord = __tmp_25 in 
+                                                let _MIRAccessFromProperty = 0 in 
+                                                    let xProjection = __tmp_30 in 
+                                                        let __tmp_31 = (Mkrecord__f_g 20 10) in 
+                                                            let xRecord2 = __tmp_31 in 
                                                                 let _MIRAccessFromProperty = 0 in 
-                                                                    let x4 = __tmp_36 in 
-                                                                        let __tmp_37 = (Mkrecord__f_g 20 10) in 
-                                                                            let x5 = __tmp_37 in 
-                                                                                let _MIRAccessFromProperty = 0 in 
-                                                                                    let x6 = __tmp_42 in 
-                                                                                        let __tmp_43 = (nSMain__identityUnion y) in 
-                                                                                            let y2 = __tmp_43 in 
-                                                                                                let __tmp_46 = (Mktuple__3 1 true 2) in 
-                                                                                                    let __tmp_45 = (nSMain__identityTupleOptional __tmp_46) in 
-                                                                                                        let z2 = __tmp_45 in 
-                                                                                                            let __tmp_51 = (Mktuple__1 "hello") in 
-                                                                                                                let __tmp_50 = (nSMain__identity __tmp_51) in 
-                                                                                                                    let z4 = __tmp_50 in 
-                                                                                                                        let __tmp_53 = (Mktuple__2 x y) in 
-                                                                                                                            let zTuple = __tmp_53 in 
-                                                                                                                                let __ir_ret__ = z in 
-                                                                                                                                    let _return_ = __ir_ret__ in 
-                                                                                                                                        _return_
+                                                                    let xProjection2 = __tmp_36 in 
+                                                                        let y = 20 in 
+                                                                            let __tmp_38 = (nSMain__identityUnion y) in 
+                                                                                let y2 = __tmp_38 in 
+                                                                                    let _MIRAccessFromIndex = 0 in 
+                                                                                        let __tmp_40 = (nSMain__max __tmp_43 y) in 
+                                                                                            let z = __tmp_40 in 
+                                                                                                let __tmp_45 = (nSMain__max z y) in 
+                                                                                                    let z_max_func_repeated = __tmp_45 in 
+                                                                                                        let __tmp_49 = (Mktuple__3 1 true 2) in 
+                                                                                                            let __tmp_48 = (nSMain__identityTupleOptional __tmp_49) in 
+                                                                                                                let z2 = __tmp_48 in 
+                                                                                                                    let __tmp_54 = (Mktuple__1 "hello") in 
+                                                                                                                        let __tmp_53 = (nSMain__identityOpenTuple __tmp_54) in 
+                                                                                                                            let z3 = __tmp_53 in 
+                                                                                                                                let __tmp_56 = (Mktuple__2 xTuple2 y) in 
+                                                                                                                                    let zTuple2 = __tmp_56 in 
+                                                                                                                                        let __ir_ret__ = z in 
+                                                                                                                                            let _return_ = __ir_ret__ in 
+                                                                                                                                                _return_
 
